Examples/LockSpec.v
@@ -1,57 +1,101 @@
 From LHL.Core Require Import
   Program
-  Specs.
+  Specs
+  UBLayer.
+
+From LHL.Util Require Import
+  Util
+  Tactics
+  TransUtil.
 
 From Coq Require Import
   Program.Equality.
+
+Require Import List.
+Import ListNotations.
 
 Variant LockSig : ESig :=
 | Acq : LockSig unit
 | Rel : LockSig unit.
 
-Variant LockState :=
-| LockDef (owner : option ThreadName) (m : option (LockSig unit))
-| LockUB.
+Variant LockState {T} :=
+| LockDef (owner : option T) (m : option (LockSig unit)).
 
-Definition LockUnowned := LockDef None None.
-Definition LockAcqRan i := LockDef (Some i) (Some Acq).
-Definition LockRelRan i := LockDef (Some i) (Some Rel).
-Definition LockOwned i := LockDef (Some i) None.
+Definition LockUnowned {T} := @LockDef T None None.
+Definition LockAcqRan {T} i := @LockDef T (Some i) (Some Acq).
+Definition LockRelRan {T} i := @LockDef T (Some i) (Some Rel).
+Definition LockOwned {T} i := @LockDef T (Some i) None.
 
-Variant LockStep : LockState -> ThreadEvent LockSig -> LockState -> Prop :=
+Variant LockStep {T} : LockState -> ThreadEvent T LockSig -> LockState -> Prop :=
 | LockCallAcq i : LockStep LockUnowned (i, CallEv Acq) (LockAcqRan i)
 | LockRetAcq i : LockStep (LockAcqRan i) (i, RetEv Acq tt) (LockOwned i)
 | LockCallRel i : LockStep (LockOwned i) (i, CallEv Rel) (LockRelRan i)
-| LockRetRel i : LockStep (LockRelRan i) (i, RetEv Rel tt) LockUnowned
-| LockUBAcq s i : s <> LockUnowned -> LockStep s (i, CallEv Acq) LockUB
-| LockUBRel s i : s <> LockOwned i -> LockStep s (i, CallEv Rel) LockUB
-| LockStepUB e : LockStep LockUB e LockUB.
+| LockRetRel i : LockStep (LockRelRan i) (i, RetEv Rel tt) LockUnowned.
 
-Program Definition lockSpec : Spec LockSig := {|
+Definition LockActiveMap {T} : ActiveF (@LockStep T) := 
+  fun s => match s with
+  | LockDef None _ => fun _ => None
+  | LockDef (Some i) (Some Acq) => 
+      fun j => if (eqb i j) then Some (existT _ _ Acq) else None
+  | LockDef (Some i) (Some Rel) =>
+      fun j => if (eqb i j) then Some (existT _ _ Rel) else None
+  | _ => fun _ => None
+  end.
+
+Lemma LockStepActiveMapStep {T} :
+  forall s1 s2 (te: @ThreadEvent T LockSig), LockStep s1 te s2 ->
+    ActiveMapStep (LockActiveMap s1) te (LockActiveMap s2).
+Proof.
+  intros.
+  inversion H; subst.
+  + econstructor; unfold LockActiveMap; simpl.
+    { reflexivity. }
+    { rewrite eqb_id. reflexivity. }
+    { apply differ_pointwise_trivial. }
+  + econstructor; unfold LockActiveMap; simpl.
+    { rewrite eqb_id. reflexivity. }
+    { reflexivity. }
+    { unfold differ_pointwise. intros. rewrite eqb_nid; easy. }
+  + econstructor; unfold LockActiveMap; simpl.
+    { reflexivity. }
+    { rewrite eqb_id. reflexivity. }
+    { apply differ_pointwise_trivial. }
+  + econstructor; unfold LockActiveMap; simpl.
+    { rewrite eqb_id. reflexivity. }
+    { reflexivity. }
+    { unfold differ_pointwise. intros. rewrite eqb_nid; easy. }
+Qed.
+
+Program Definition lockSpec {T} : Spec T LockSig := {|
   State := LockState;
   Step := LockStep;
   Init := LockUnowned
 |}.
 
-Admit Obligations.
-
-Definition OwnsLock i s :=
-  match s with
-  | LockDef (Some j) _ => i = j
-  | _ => False
-  end.
-
-Definition owner s :=
-  match s with
-  | LockDef o _ => o
-  | LockUB => None
-  end.
-
-Lemma owner_correct :
-  forall s i, owner s = Some i <-> OwnsLock i s.
-unfold owner, OwnsLock. intros.
-split; intros.
-destruct s; subst; easy.
-destruct s. destruct owner0; subst; easy.
-contradiction.
+Next Obligation.
+  intros.
+  change (fun _ : Name T => None) with ((@LockActiveMap T) LockUnowned).
+  generalize dependent (@LockUnowned (Name T)).
+  induction p; intros.
+  + constructor.
+  + inversion H; subst.
+    specialize (IHp st'' H4).
+    pose proof LockStepActiveMapStep l st'' a H2.
+    apply (ActiveMapStepSeqcons _ _ _ _ H0 IHp).
 Qed.
+
+Global Lemma LockActiveMapSound {T} : @acf_sound T LockSig lockSpec LockActiveMap.
+Proof.
+  split.
+  + reflexivity.
+  + intros.
+    apply LockStepActiveMapStep, H.
+Qed.
+
+
+Definition lockClientSpec {T} : forall A, LockSig A -> Name T -> LockState -> Prop :=
+  fun A m i s => 
+    match m with
+    | Acq => (s <> LockOwned i) /\ (s <> LockAcqRan i) /\ (s <> LockRelRan i)
+    | Rel => s = LockOwned i
+    end.
