Examples/SpinLock.v
@@ -1,0 +1,1512 @@
+From LHL.Core Require Import
+  Program
+  ProgramRules
+  Specs
+  Logic
+  Tensor
+  Traces
+  Linearizability
+  UBLayer2.
+
+From LHL.Examples Require Import
+  LockSpec
+  CASSpec
+  LocalVarSpec.
+
+From LHL.Util Require Import
+  Tactics
+  TransUtil
+  Util.
+
+From Coq Require Import
+  Logic.FunctionalExtensionality
+  Logic.PropExtensionality
+  Program.Equality.
+
+Definition SpinLockAcq : Prog (CASSig bool) unit :=
+  while (tmp <- call (CAS None (Some true)); ret (negb tmp)) skip.
+
+Definition SpinLockRel: Prog (CASSig bool) unit :=
+  call (CAS (Some true) None);;
+  ret tt.
+
+Definition SpinLockImpl: Impl (CASSig bool) LockSig :=
+  fun _ m =>
+    match m with
+    | Acq => SpinLockAcq
+    | Rel => SpinLockRel
+    end.
+
+Definition E := CASSig bool.
+Definition F := LockSig.
+Definition acf T := @LockActiveMap T.
+Definition HAcf T : @acf_sound T F lockSpec (acf T) := @LockActiveMapSound T.
+Definition VE T : Spec T E:= @casSpec T bool.
+Definition VF T := @lockSpec T.
+Definition VFU T := SpecWithUB (@lockSpec T) (acf T) (HAcf T).
+Definition ReltU T := Relt (VE T) (VFU T).
+Definition Relt T := Relt (VE T) (VF T).
+Definition PrecU T := Prec (VE T) (VFU T).
+Definition Prec T := Prec (VE T) (VF T).
+Definition PostU T := Post (VE T) (VFU T).
+Definition Post T := Post (VE T) (VF T).
+Definition UState T := State (VFU T).
+
+Definition Precs {T} i A (m : LockSig A) : @PrecU T :=
+  fun s ρs => exists ρ, ρs = eq ρ /\
+    match m with
+    | Acq =>
+        True (* To be complete *)
+    | Rel =>
+        (PState ρ = inl (LockOwned i) /\ snd s = CASDef (Some true) None) \/
+        (PState ρ <> inl (LockOwned i) /\ (StateWithUB_acf _ (acf T) (PState ρ) i = None))
+    end.
+
+Definition Posts {T} i A (m : LockSig A) : @PostU T A :=
+  fun v s ρs t σs => exists ρ σ, ρs = eq ρ /\ σs = eq σ /\
+    match m with
+    | Acq =>
+        True (* To be complete *)
+    | Rel =>
+        PCalls σ i = CallDone Rel /\
+        PRets σ i = RetPoss Rel tt /\
+        ((PState ρ = inl (LockOwned i) /\ (forall m, PState σ <> inl (LockDef (Some i) m)) /\ fst t i = Cont m (Return v)) \/
+         (exists a, PState σ = inr (UBState_, a)))
+    end.
+
+Module SpinLockNormal.
+
+(* Definition E := CASSig bool.
+Definition F := LockSig.
+Definition VE T : Spec T E:= @casSpec T bool.
+Definition VF T := @lockSpec T.
+Definition Relt T := Relt (VE T) (VF T).
+Definition Prec T := Prec (VE T) (VF T).
+Definition Post T := Post (VE T) (VF T). *)
+
+(* Definition Valid {T} : Prec T :=
+  fun s ρs => exists ρ, ρs = eq ρ /\
+    ((PState ρ = LockUnowned /\ exists m, snd s = CASDef None m) \/
+    (exists j, PState ρ = LockAcqRan j /\ exists m, snd s = CASDef None m) \/
+    (exists j, PState ρ = LockOwned j /\ exists m, snd s = CASDef (Some true) m) \/
+    (exists j, PState ρ = LockRelRan j /\ exists m, snd s = CASDef (Some true) m)).
+
+Definition Invalid {T} : Prec T :=
+  fun s ρs => ~Valid s ρs. *)
+
+Definition Precs {T} i A (m : LockSig A) : Prec T :=
+  fun s ρs => exists ρ, ρs = eq ρ /\
+    match m with
+    | Acq =>
+        (PState ρ <> LockOwned i /\ PState ρ <> LockRelRan i /\ PState ρ <> LockAcqRan i)
+    | Rel =>
+        PState ρ = LockOwned i /\ snd s = CASDef (Some true) None
+    end.
+
+Definition Posts {T} i A (m : LockSig A) : Post T A :=
+  fun v s ρs t σs => exists ρ σ, ρs = eq ρ /\ σs = eq σ /\
+    match m with
+    | Acq =>
+        (PState σ = LockOwned i /\ PState ρ <> LockOwned i)
+    | Rel =>
+        PState ρ = LockOwned i /\
+        (forall m, PState σ <> LockDef (Some i) m) /\
+        σ.(PRets) i = RetPoss m v /\
+        σ.(PCalls) i = CallDone m /\
+        fst t i = Cont m (Return v)
+    end.
+
+Definition Rely {T} i : Relt T :=
+  fun s ρs t σs => forall ρ, ρs = eq ρ -> exists σ, σs = eq σ /\
+    (PCalls ρ i = PCalls σ i) /\
+    (PRets ρ i = PRets σ i) /\
+    (forall m, PState ρ = LockDef (Some i) m -> PState σ = LockDef (Some i) m) /\ 
+    (forall m, PState ρ = LockDef (Some i) m -> snd s = snd t) /\
+    ((forall m, PState ρ <> LockDef (Some i) m) -> (forall m, PState σ <> LockDef (Some i) m)) /\
+    (fst s i = fst t i).
+
+Definition Guar {T} i : Relt T :=
+  fun s ρs t σs => forall ρ, ρs = eq ρ -> exists σ, σs = eq σ /\
+    (forall j, j <> i -> fst s j = fst t j) /\
+    (forall j, j <> i -> PCalls ρ j = PCalls σ j) /\
+    (forall j, j <> i -> PRets ρ j = PRets σ j) /\
+    (forall j, j <> i -> 
+      forall m, PState ρ = LockDef (Some j) m -> PState σ = LockDef (Some j) m) /\
+    (forall j, j <> i -> 
+      forall m, PState ρ = LockDef (Some j) m -> snd s = snd t) /\
+    (forall j, j <> i -> 
+      ((forall m, PState ρ <> LockDef (Some j) m) -> (forall m, PState σ <> LockDef (Some j) m))).
+
+Lemma SpinLock_R_refl {T} : forall (i : Name T) s ρ, Rely i s ρ s ρ.
+Proof.
+  unfold Rely; intros.
+  exists ρ0.
+  split; auto.
+  repeat split; intros; auto.
+Qed.
+
+Lemma SpinLock_R_trans {T} : 
+  forall (i : Name T), Rely i ->> Rely i ==> Rely i.
+Proof.
+  unfold sub, subRelt.
+  intros.
+  unfold ReltCompose in H.
+  destruct_all.
+  rename x into s'.
+  rename x0 into ρ'.
+  unfold Rely in *.
+  intros.
+  specialize (H ρ0 H1).
+  destruct_all.
+  rename x into ρ'_.
+  specialize (H0 ρ'_ H).
+  destruct_all.
+  rename x into σ_.
+  exists σ_.
+  repeat split; intros; try easy.
+Admitted.
+
+Lemma SpinLock_G_in_R {T} : 
+  forall (i j : Name T), i <> j -> Guar i ==> Rely j.
+Proof.
+  unfold Guar, Rely, sub, subRelt. intros.
+  specialize (H0 _ H1).
+  destruct_all.
+  exists x.
+  specialize (H2 j (ltac: (easy))).
+  specialize (H3 j (ltac: (easy))).
+  specialize (H4 j (ltac: (easy))).
+  specialize (H5 j (ltac: (easy))).
+  specialize (H6 j (ltac: (easy))).
+  specialize (H7 j (ltac: (easy))).
+  repeat split; intros; try easy.
+  + specialize (H5 m).
+    apply H5, H8.
+  + specialize (H5 m).
+    apply (H6 _ H8).
+  + apply H7, H8.
+Qed.
+
+Lemma Poss_eq_inv: forall {T A VF} (i: Name T) (m : LockSig A) ρs ρ σs (σ: Poss VF),
+  ρs = eq ρ ->
+  σs = (fun σ  =>
+        exists ρ,
+        ρs ρ /\
+        PState σ = PState ρ /\
+        PCalls σ i = CallPoss m /\
+        PRets σ i = RetIdle /\
+        differ_pointwise (PCalls ρ) (PCalls σ) i /\
+        differ_pointwise (PRets ρ) (PRets σ) i) ->
+  σ = {| PState := PState ρ; PCalls :=
+        fun k : Name T =>
+          if i =? k then CallPoss m 
+          else PCalls ρ k; PRets :=
+        fun k : Name T =>
+          if i =? k then RetIdle 
+          else PRets ρ k |} ->
+  σs = eq σ.
+Proof.
+  intros.
+  rewrite H0, H1.
+  extensionality σ'.
+  apply propositional_extensionality.
+  split.
+  { 
+    clear H0 H1.
+    intros.
+    destruct H0 as [ρ' [? [? [? [? [? ?]]]]]].
+    assert(ρ = ρ'). { rewrite H in H0. apply H0. }
+    subst ρ'.
+    destruct σ'; simpl in *.
+    apply f_equal3.
+    { auto. }
+    { 
+      extensionality k. destruct (classicT (i = k)).
+      { subst k. rewrite eqb_id. auto. }
+      { 
+        rewrite (eqb_nid _ _ n).
+        unfold differ_pointwise in H4.
+        specialize (H4 k (ltac:(auto))).
+        auto.
+      }
+    }
+    { 
+      extensionality k. destruct (classicT (i = k)).
+      { subst k. rewrite eqb_id. auto. }
+      { 
+        rewrite (eqb_nid _ _ n).
+        unfold differ_pointwise in H5.
+        specialize (H5 k (ltac:(auto))).
+        auto.
+      }
+    }
+  }
+  {
+    intros. subst σ'.
+    exists ρ.
+    repeat split.
+    { rewrite H. reflexivity. }
+    { simpl. rewrite eqb_id. reflexivity. } 
+    { simpl. rewrite eqb_id. reflexivity. }
+    { simpl. apply differ_pointwise_trivial. }
+    { simpl. apply differ_pointwise_trivial. }
+  }
+Qed.
+
+Lemma Poss_eq_inv2: forall {T A VF} (i: Name T) (m : LockSig A) ρs ρ (σs: PossSet VF),
+  ρs = eq ρ ->
+  σs = (fun σ =>
+        exists ρ,
+        ρs ρ /\
+        PState σ = PState ρ /\
+        PCalls σ i = CallPoss m /\
+        PRets σ i = RetIdle /\
+        differ_pointwise (PCalls ρ) (PCalls σ) i /\
+        differ_pointwise (PRets ρ) (PRets σ) i) ->
+  σs = eq {| PState := PState ρ; PCalls :=
+        fun k : Name T =>
+          if i =? k then CallPoss m 
+          else PCalls ρ k; PRets :=
+        fun k : Name T =>
+          if i =? k then RetIdle 
+          else PRets ρ k |}.
+Proof.
+  intros.
+  pose proof Poss_eq_inv i m ρs ρ σs 
+    {| PState := PState ρ; 
+       PCalls := fun j : Name T => if i =? j then CallPoss m else PCalls ρ j; 
+       PRets := fun j : Name T => if i =? j then RetIdle else PRets ρ j |} H H0.
+    apply H1.
+    reflexivity.
+Qed.
+
+Lemma Poss_eq_inv3: forall {F T} {VF: Spec T F} (i: Name T) (ρ: Poss VF) σs (st: State VF) pcall pret,
+  σs = (fun σ =>
+        PState σ = st /\
+        PCalls σ i = pcall /\
+        PRets σ i = pret /\
+        differ_pointwise (PCalls ρ) (PCalls σ) i /\
+        differ_pointwise (PRets ρ) (PRets σ) i) ->
+  σs = eq ( {| PState := st; 
+        PCalls := fun k : Name T => if i =? k then pcall else PCalls ρ k; 
+        PRets :=  fun k : Name T => if i =? k then pret else PRets ρ k |} : Poss VF).
+Proof.
+  intros.
+  extensionality σ'.
+  apply propositional_extensionality.
+  split.
+  { 
+    intros.
+    rewrite H in H0.
+    destruct H0 as [? [? [? [? ?]]]].
+    destruct σ'; simpl in *.
+    unfold differ_pointwise in H3, H4.
+    f_equal; try easy.
+    { extensionality k.
+      destruct (classicT (i = k)).
+      { subst k. rewrite eqb_id. auto. }
+      { rewrite (eqb_nid _ _ n). specialize (H3 k (ltac:(auto))). auto. }
+    }
+    { extensionality k.
+      destruct (classicT (i = k)).
+      { subst k. rewrite eqb_id. auto. }
+      { rewrite (eqb_nid _ _ n). specialize (H4 k (ltac:(auto))). auto. }
+    }
+  }
+  {
+    intros.
+    subst σ'.
+    rewrite H.
+    simpl.
+    rewrite eqb_id.
+    repeat split; auto.
+    { apply differ_pointwise_trivial. }
+    { apply differ_pointwise_trivial. }
+  }
+Qed.
+
+Lemma Poss_eq_unique: forall {T} ρs (ρ: Poss (VF T)) ρ', 
+  ρs = eq ρ -> ρs ρ' -> ρ = ρ'.
+Proof.
+  intros.
+  rewrite H in H0.
+  apply H0.
+Qed.
+
+Lemma Poss_eq_unique2: forall {T} ρs (ρ: Poss (VF T)) ρ', 
+  ρs = eq ρ -> ρs = eq ρ' -> ρ' = ρ.
+Proof.
+  intros.
+  rewrite H in H0.
+  assert(eq ρ ρ = eq ρ' ρ). { rewrite H0. reflexivity. }
+  rewrite <- H1.
+  reflexivity.
+Qed.
+
+Lemma SpinLock_Inv_in_R {T} : 
+  forall (i j : Name T), i <> j -> InvokeAny SpinLockImpl i ==> Rely j.
+Proof.
+  unfold InvokeAny, Guar, Rely, sub, subRelt; intros.
+  rename σ into σs.
+  rename ρ into ρs.
+  rename ρ0 into ρ.
+  destruct H0 as [Ret [m HInv]].
+  unfold TInvoke in HInv.
+  destruct HInv as [HIdle [HO [HU Hsig]]].
+  set ( σ :=
+     {| 
+        PState := ρ.(PState); 
+        PCalls := fun k =>
+          if (eqb i k) then CallPoss m
+          else ρ.(PCalls) k;
+        PRets := fun k =>
+          if (eqb i k) then RetIdle
+          else ρ.(PRets) k 
+      |}).
+  exists σ.
+  pose proof Poss_eq_inv i m ρs ρ σs σ H1 Hsig (ltac:(reflexivity)) as H0.
+  repeat split; simpl; try rewrite (eqb_nid _ _ H); auto.
+  inversion HO; exact (H3 j (ltac:(auto))).
+Qed.
+
+Lemma SpinLock_Ret_in_R {T} : 
+  forall (i j : Name T), i <> j -> ReturnAny SpinLockImpl i ==> Rely j.
+Proof.
+  unfold ReturnAny, Guar, Rely, sub, subRelt; intros.
+  rename σ into σs.
+  rename ρ into ρs.
+  rename ρ0 into ρ.
+  destruct H0 as [Ret [m HRet]].
+  unfold TReturn in HRet.
+  destruct HRet as [v [? [? [? ?]]]].
+  set ( σ :=
+     {| 
+        PState := ρ.(PState); 
+        PCalls := fun k =>
+          if (eqb i k) then CallDone m
+          else ρ.(PCalls) k;
+        PRets := fun k =>
+          if (eqb i k) then RetPoss m v
+          else ρ.(PRets) k 
+      |}).
+  exists σ.
+  unfold mapRetPoss in H4.
+  repeat split; simpl; try rewrite (eqb_nid _ _ H); auto.
+  + rewrite H4.
+    extensionality x.
+    apply propositional_extensionality.
+    admit.
+  + inversion H2.
+    exact (H6 j (ltac:(auto))).
+Admitted.
+
+(* Lemma SpinLock_init_in_P {T} : 
+  forall i (A: Type) m, Precs i A m (allIdle, (VE T).(Init)) (eq initPoss).
+Proof.
+  intros.
+  unfold Precs.
+  exists initPoss. split; auto.
+  destruct m; simpl; intros; try easy.
+  split. *)
+
+Lemma SpinLock_P_stable {T} : 
+  forall (i: Name T) A m, Stable (Rely i) (Precs i A m).
+Proof.
+  unfold Stable, stablePrec, PrecCompose, sub, subPrec.
+  intros.
+  destruct H as [s0 [ρ0 [? ?]]].
+  unfold Precs in *.
+  unfold Rely in H0.
+  destruct m.
+  + destruct H as [ρ0' [? ?]].
+    specialize (H0 _ H).
+    destruct H0 as [ρ' [? ?]].
+    exists ρ'. split; auto.
+    destruct_all.
+    assert((forall m : option(LockSig unit), PState ρ0' <> LockDef (Some i) m)). {
+      intros.
+      unfold LockOwned, LockRelRan, LockAcqRan in *.
+      destruct m; try easy.
+      dependent destruction l; easy.
+    }
+    specialize (H6 H10).
+    pose proof (H10 None).
+    pose proof (H10 (Some Rel)).
+    pose proof (H10 (Some Acq)).
+    unfold LockOwned, LockRelRan, LockAcqRan.
+    repeat split; easy.
+  + destruct H as [ρ0' [? ?]].
+    specialize (H0 _ H).
+    destruct H0 as [ρ' [? ?]].
+    exists ρ'. split; auto.
+    destruct_all.
+    specialize (H4 None).
+    specialize (H4 H1).
+    split; [exact H4 | ].
+    assert(snd s0 = snd s). {
+      specialize (H5 None).
+      apply H5, H1.
+    }
+    rewrite <- H9.
+    apply H8.
+Qed.
+
+(* Lemma SpinLock_Q_stable {T} : 
+  forall (i: Name T) A m, Stable (Rely i) (Posts i A m).
+Proof.
+  unfold Stable, stablePost, stableRelt, sub, subRelt, ReltCompose.
+  intros.
+  destruct H as [t0 [σ0 [? ?]]].
+  unfold Posts in *.
+  unfold Rely in H0.
+  intros.
+  specialize (H _ H1).
+  destruct H as [σ0' [? ?]].
+  specialize (H0 _ H).
+  destruct H0 as [σ' [? ?]].
+  exists σ'. split; [exact H0 | ].
+  destruct m.
+  + destruct_all.
+    specialize (H5 None).
+    pose proof (proj1 H5 H2).
+    easy.
+  + destruct_all.
+    specialize (H5 None).
+    pose proof (proj1 H5).
+    repeat split; try easy.
+    { apply (proj1 H7 H9). }
+    { rewrite <- H4. apply H10. }
+    { rewrite <- H3. apply H11. }
+    { rewrite <- H12, H8. reflexivity. }
+Qed. *)
+
+(* Lemma SpinLock_switch_code {T} : 
+  forall (i: Name T) A m1 B m2 v,
+    (prComp (Precs i A m1) (Posts i A m1 v)) <<- (Posts i A m1 v) <<- TReturn SpinLockImpl i m1 v ==> Precs i B m2.
+Proof.
+  intros.
+  unfold sub, subPrec, subRelt, ReltCompose, PrecCompose.
+  intros.
+  destruct H as [s1 [ρ1 [? ?]]].
+  destruct H as [s2 [ρ2 [? ?]]].
+Admitted. *)
+
+Lemma Rel_verify_aux' {T} :
+  forall (i: Name T) (s0: InterState F (VE T)) (ρs0: PossSet (VF T)) s1 ρs1,
+    (prComp (Precs i unit Rel) (TInvoke SpinLockImpl i unit Rel)) s0 ρs0 s1 ρs1 ->
+      exists ρ1, ρs1 = eq ρ1 /\
+        PState ρ1 = LockOwned i /\
+        PCalls ρ1 i = CallPoss Rel /\
+        PRets ρ1 i = RetIdle /\
+        snd s1 = CASDef (Some true) None /\  
+        fst s1 i = Cont Rel (SpinLockImpl _ Rel).
+Proof.
+  intros.
+  unfold prComp, ReltCompose in H.
+  destruct H.
+  unfold Precs in H.
+  destruct H as [ρ [? [? ?]]].
+  unfold TInvoke in H0.
+  destruct H0 as [? [? [? ?]]].
+  exists {| 
+    PState := ρ.(PState); 
+    PCalls := fun j =>
+      if (eqb i j) then CallPoss Rel
+      else ρ.(PCalls) j;
+    PRets := fun j =>
+      if (eqb i j) then RetIdle
+      else ρ.(PRets) j
+  |}.
+  simpl.
+  rewrite (eqb_id i).
+  rewrite <- H2.
+  unfold TIdle in H0.
+  destruct H0.
+  split.
+  { pose proof Poss_eq_inv i Rel ρs0 ρ ρs1 
+    {| PState := PState ρ; 
+       PCalls := fun j : Name T => if i =? j then CallPoss Rel else PCalls ρ j; 
+       PRets := fun j : Name T => if i =? j then RetIdle else PRets ρ j |} H H5.
+    apply H7.
+    reflexivity. }
+  repeat split; try easy.
+  inversion H3; subst; simpl in *.
+  inversion H7; subst.
+  dependent destruction H5.
+  exact H12.
+Qed.
+
+Lemma Rel_verify_aux {T} :
+  forall (i: Name T) (s0: InterState F (VE T)) (ρs0: PossSet (VF T)) s1 ρs1,
+    (prComp (Precs i unit Rel) (TInvoke SpinLockImpl i unit Rel) ->> Rely i) s0 ρs0 s1 ρs1 ->
+      exists ρ1, ρs1 = eq ρ1 /\
+        PState ρ1 = LockOwned i /\
+        PCalls ρ1 i = CallPoss Rel /\
+        PRets ρ1 i = RetIdle /\
+        snd s1 = CASDef (Some true) None /\  
+        fst s1 i = Cont Rel (SpinLockImpl _ Rel).
+Proof.
+  intros.
+  unfold ReltCompose in H.
+  destruct H as [s2 [ρs2 [? ?]]].
+  pose proof Rel_verify_aux' i s0 ρs0 s2 ρs2 H.
+  destruct H1 as [ρ2 [? [? [? [? [? ?]]]]]].
+  unfold Rely in H0.
+  specialize (H0 _ H1).
+  destruct H0 as [ρ1 [? ?]].
+  destruct_all.
+  exists ρ1.
+  split; [exact H0 | ].
+  split; [apply (H9 None H2) |].
+  split.
+  { rewrite <- H7. apply H3. }
+  split.
+  { rewrite <- H8. apply H4. }
+  split. 
+  { pose proof (H10 None H2). rewrite <- H13. apply H5. }
+  rewrite <- H12. apply H6.
+Qed.
+
+Lemma Rel_verify_aux'' {T} :
+  forall (i: Name T) (s0: InterState F (VE T)) (ρs0: PossSet (VF T)) s1 ρs1,
+    (prComp (Precs i unit Rel) (TInvoke SpinLockImpl i unit Rel) ->> Rely i) s0 ρs0 s1 ρs1 ->
+      exists ρ0, ρs0 = eq ρ0 /\ PState ρ0 = LockOwned i /\ snd s0 = CASDef (Some true) None.
+Proof.
+  intros.
+  unfold prComp, ReltCompose in H.
+  destruct_all.
+  unfold Precs in H.
+  unfold PrecToRelt in H.
+  apply H.
+Qed.
+
+Lemma differ_pointwise_trans {A State} : forall (i: A) s1 s2 (s3: (A -> State)),
+  differ_pointwise s1 s2 i -> differ_pointwise s2 s3 i -> differ_pointwise s1 s3 i.
+Proof.
+  intros.
+  unfold differ_pointwise in *.
+  intros.
+  specialize (H j H1).
+  specialize (H0 j H1).
+  auto.
+  rewrite H0, H.
+  reflexivity.
+Qed.
+
+Lemma SpinLock_Rel_verified {T} : 
+  forall (i: Name T),
+    VerifyProg i (Rely i) (Guar i)
+      (prComp (Precs i unit Rel) (TInvoke SpinLockImpl i _ Rel) ->> Rely i)
+      (SpinLockImpl _ Rel)
+      (fun v => Posts i unit Rel v).
+Proof.
+  intros. simpl.
+  unfold SpinLockRel.
+  apply (lemBind (fun (_: bool) => 
+            (fun v : unit => Posts i unit Rel v) tt)).
+  + eapply weakenPost.
+    eapply (lemCall 
+      (Q := fun (s: InterState F (VE T)) (ρs: PossSet (VF T)) t σs =>
+        exists ρ σ, ρs = eq ρ /\ σs = eq σ /\
+        UnderThreadStep (fst s i) (Some (CallEv (CAS (Some true) None))) (fst t i) /\
+        Step (VE T) (snd s) (i, (CallEv (CAS (Some true) None))) (snd t) /\ 
+        PState σ = LockRelRan i /\
+        PCalls σ i = CallDone Rel /\
+        PRets σ i = RetIdle /\
+        True /\ True)   (* The following conditions are removed. Use True /\ True to avoid label changes  *)
+        (* (forall j, j <> i -> PCalls σ j = PCalls ρ j) /\
+        (forall j, j <> i -> PRets σ j = PRets ρ j)) *)
+      (S := fun v s ρs t σs =>
+        exists ρ σ, ρs = eq ρ /\ σs = eq σ /\ v = true /\
+        UnderThreadStep (fst s i) (Some (RetEv (CAS (Some true) None) true)) (fst t i) /\
+        (forall m, PState σ <> LockDef (Some i) m) /\
+        PCalls σ i = CallDone Rel /\
+        PRets σ i = RetPoss Rel tt /\
+        True /\ True)).   (* The following conditions are removed. Use True /\ True to avoid label changes  *)
+        (* (forall j, j <> i -> PCalls σ j = PCalls ρ j) /\
+        (forall j, j <> i -> PRets σ j = PRets ρ j))). *)
+    {
+      unfold Stable, stableRelt, sub, subRelt.
+      intros; simpl in *.
+      unfold ReltCompose in H.
+      rename ρ into ρs.
+      rename σ into σs.
+      destruct H as [s0 [ρs0 [? ?]]].
+      destruct H as [ρ [ρ0 [? [? ?]]]].
+      unfold Rely in H0.
+      specialize (H0 _ H1).
+      destruct H0 as [σ [? ?]].
+      exists ρ, σ.
+      split; [exact H |].
+      split; [exact H0 |].
+      destruct_all.
+      change (@fst (ThreadsSt T E F) (CASState T bool) t i) with 
+        (@fst (ThreadsSt T E LockSig) (@State T E (VE T)) t i).
+      rewrite <- H8.
+      split; [exact H2 |].
+      specialize (H6 _ H10).
+      change (@snd (ThreadsSt T E F) (CASState T bool) t) with 
+        (@snd (ThreadsSt T E LockSig) (@State T E (VE T)) t).
+      rewrite <- H6.
+      split; [ exact H9 |].
+      split; [ apply (H5 (Some Rel) H10) |].
+      split.
+      { unfold F in H11. rewrite H11 in H3. unfold F. rewrite H3. reflexivity. }
+      split.
+      { unfold F in H12. rewrite H12 in H4. unfold F. rewrite H4. reflexivity. }
+      easy.
+    }
+    { 
+      unfold Stable, stablePost, stableRelt, sub, subRelt.
+      intros; simpl in *.
+      unfold ReltCompose in H.
+      rename ρ into ρs.
+      rename σ into σs.
+      destruct H as [s0 [ρs0 [? ?]]].
+      destruct H as [ρ [ρ0 [? [? ?]]]].
+      unfold Rely in H0.
+      specialize (H0 _ H1).
+      destruct H0 as [σ [? ?]].
+      exists ρ, σ.
+      split; [exact H |].
+      split; [exact H0 |].
+      destruct_all.
+      split; [exact H2 |].
+      change (@fst (ThreadsSt T E F) (CASState T bool) t i) with 
+        (@fst (ThreadsSt T E LockSig) (@State T E (VE T)) t i).
+      rewrite <- H8.
+      split; [exact H9 |].
+      split; [apply H7, H10 |].
+      split.
+      { unfold F in H11. rewrite H11 in H3. unfold F. rewrite H3. reflexivity. }
+      split.
+      { unfold F in H12. rewrite H12 in H4. unfold F. rewrite H4. reflexivity. }
+      easy.
+    }
+    { 
+      unfold Commit.
+      intros.
+      unfold ReltToPrec in H.
+      destruct H as [s0 [ρs0 ?]].
+      pose proof Rel_verify_aux i s0 ρs0 s ρs H.
+      destruct H3 as [ρ [? ?]].
+      destruct_all.
+      remember
+      (fun σ: Poss (VF T) => 
+        PState σ = LockRelRan i /\
+        PCalls σ i = CallDone Rel /\
+        PRets σ i = RetIdle /\
+        differ_pointwise (PCalls ρ) (PCalls σ) i /\
+        differ_pointwise (PRets ρ) (PRets σ) i) as σs.
+      pose proof Poss_eq_inv3 _ _ _ _ _ _ Heqσs.
+      remember (
+        (MkPoss T LockSig (VF T)
+        (@LockRelRan (Name T) i)
+        (fun k : Name T =>
+      match @eqb (Name T) i k
+      return (PCall LockSig) with
+      | true => @CallDone LockSig unit Rel
+      | false => @PCalls T LockSig (VF T) ρ k
+      end)
+        (fun k : Name T =>
+      match @eqb (Name T) i k
+      return (PRet LockSig) with
+      | true => @RetIdle LockSig
+      | false => @PRets T LockSig (VF T) ρ k
+      end))) as σ.
+      exists σs.
+      split. { exists σ. rewrite H9. reflexivity. }
+      split. 
+      { intros. exists ρ. 
+        pose proof Poss_eq_unique _ _ _ H9 H10; subst σ0. 
+        split. { rewrite H3. reflexivity. }
+        apply (PossStepsStep i ρ σ σ).
+        { apply (PCommitCall i _ _ unit Rel); subst σ; simpl; try easy.
+          { rewrite H4. constructor. }
+          { rewrite eqb_id. reflexivity. }
+          { rewrite eqb_id. reflexivity. }
+        }
+        { intros. subst σ. simpl. rewrite (eqb_nid _ _ H11). reflexivity. }
+        { intros. subst σ. simpl. rewrite (eqb_nid _ _ H11). reflexivity. }
+        { constructor. }
+      }
+      split.
+      { exists ρ, σ.
+        repeat split; subst σ; simpl; try rewrite eqb_id; try easy.
+        (* { intros. rewrite (eqb_nid i j (ltac:(auto))). reflexivity. }
+        { intros. rewrite (eqb_nid i j (ltac:(auto))). reflexivity. } *)
+      }
+      unfold Guar.
+      intros.
+      pose proof Poss_eq_unique2 _ _ _ H3 H10; subst ρ0.
+      exists σ.
+      split; [exact H9 |].
+      unfold differ_pointwise in H0.
+      split. { intros. specialize (H0 _ H11); easy. }
+      split.
+      { intros. subst σ. simpl. rewrite (eqb_nid i j (ltac:(auto))). reflexivity. }
+      split.
+      { intros. subst σ. simpl. rewrite (eqb_nid i j (ltac:(auto))). reflexivity. }
+      split.
+      { intros. subst σ; simpl. rewrite H4 in H12. inversion H12; subst j; contradiction. }
+      split.
+      { intros. subst σ; simpl.
+        rewrite H4 in H12. inversion H12; subst j; contradiction. }
+      intros.
+      subst σ; intros; simpl.
+      { unfold LockRelRan. intro. inversion H13; subst; contradiction. }
+    }
+    {
+      unfold Commit; intros.
+      unfold ReltToPrec in H.
+      destruct H as [s0 [ρs0 ?]].
+      unfold ReltCompose in H at 1.
+      destruct H as [s1 [ρs1 ?]].
+      destruct H.
+      pose proof Rel_verify_aux i s0 ρs0 s1 ρs1 H.
+      clear H.
+      destruct H4 as [ρ1 [? ?]].
+      destruct_all.
+      assert(ρ1 = x). { apply (Poss_eq_unique2 _ _ _ H3 H). }
+      subst x.
+      rename x0 into ρ.
+      remember
+      (fun σ: Poss (VF T) => 
+        PState σ = LockUnowned /\
+        PCalls σ i = CallDone Rel /\
+        PRets σ i = RetPoss Rel tt /\
+        differ_pointwise (PCalls ρ) (PCalls σ) i /\
+        differ_pointwise (PRets ρ) (PRets σ) i) as σs.
+      pose proof Poss_eq_inv3 _ _ _ _ _ _ Heqσs.
+      remember
+      (MkPoss T LockSig (VF T) (@LockUnowned (Name T))
+      (fun k : Name T =>
+      match @eqb (Name T) i k return (PCall LockSig) with
+      | true => @CallDone LockSig unit Rel
+      | false => @PCalls T LockSig (VF T) ρ k
+      end)
+        (fun k : Name T =>
+      match @eqb (Name T) i k return (PRet LockSig) with
+      | true => @RetPoss LockSig unit Rel tt
+      | false => @PRets T LockSig (VF T) ρ k
+      end)) as σ.
+      exists σs.
+      split. { exists σ. rewrite H17; reflexivity. } 
+      split.
+      { intros. pose proof Poss_eq_unique _ _ _ H17 H18; subst σ0. 
+        exists ρ. split; [rewrite H9; reflexivity |].
+        apply (PossStepsStep i ρ σ σ).
+        { apply (PCommitRet i _ _ unit Rel tt); subst σ; simpl; try easy.
+          { unfold F in H12. rewrite H12. constructor. }
+          { rewrite eqb_id. reflexivity. }
+          { rewrite eqb_id. reflexivity. }
+        }
+        { intros. subst σ. simpl. rewrite (eqb_nid _ _ H19). reflexivity. }
+        { intros. subst σ. simpl. rewrite (eqb_nid _ _ H19). reflexivity. }
+        { constructor. }
+      }
+      split.
+      { exists ρ, σ.
+        assert(v = true).
+        { unfold F in H11.
+          rewrite H7 in H11.
+          inversion H11; subst.
+          change (@snd (ThreadsSt T E F) (@State T E (VE T)) s) with 
+            (@snd (ThreadsSt T E LockSig) (CASState T bool) s) in H2.
+          rewrite <- H23 in H2.
+          inversion H2; subst.
+          { dependent destruction H21; easy. }
+          { contradiction. }
+        }
+        subst v.
+        repeat split; subst σ; simpl; try rewrite eqb_id; try easy.
+        (* { intros. rewrite (eqb_nid i j (ltac:(auto))). reflexivity. }
+        { intros. rewrite (eqb_nid i j (ltac:(auto))). reflexivity. } *)
+      }
+      unfold Guar.
+      intros.
+      pose proof Poss_eq_unique2 _ _ _ H18 H9; subst ρ0.
+      exists σ.
+      split; [exact H17 |]. 
+      split.
+      { unfold differ_pointwise in H0. intros. specialize (H0 _ H19); easy. }
+      split.
+      { subst σ. simpl. intros. rewrite (eqb_nid i j (ltac:(auto))). reflexivity. }
+      split.
+      { subst σ. simpl. intros. rewrite (eqb_nid i j (ltac:(auto))). reflexivity. }
+      split.
+      { subst σ. simpl. unfold F in H12. rewrite H12.
+        intros; inversion H20; subst j; contradiction. }
+      split.
+      { subst σ. simpl. unfold F in H12. rewrite H12. intros. inversion H20; subst j; contradiction. }
+      intros.
+      subst σ; intros; simpl.
+      { unfold LockUnowned. intro. inversion H21; subst; contradiction. }
+    }
+    {
+      unfold sub, subRelt.
+      intros.
+      unfold ReltToPrec in H.
+      rename ρ into ρs.
+      rename σ into σs.
+      destruct H as [s0 [ρs0 ?]].
+      unfold ReltCompose in H at 2.
+      destruct H.
+      pose proof Rel_verify_aux i s ρs s0 ρs0 H.
+      destruct H1 as [ρ0 [? ?]].
+      destruct H0 as [s1 [ρs1 ?]].
+      destruct H0.
+      destruct H0 as [ρ0_ [ρ1 [? [? ?]]]].
+      pose proof Poss_eq_unique2 _ _ _ H0 H1; subst ρ0_.
+      destruct H3 as [ρ1_ [σ [? [? ?]]]].
+      pose proof Poss_eq_unique2 _ _ _ H3 H4; subst ρ1_.
+      unfold Posts. intros.
+      pose proof Rel_verify_aux'' i s ρs s0 ρs0 H.
+      destruct H8 as [ρ [? ?]].
+      exists ρ, σ.
+      split; [exact H8 |].
+      split; [exact H6 |].
+      split; [exact (proj1 H9) |].
+      destruct_all.
+      split; [exact H16 |].
+      split; [exact H18|].
+      split; [exact H17 |].
+      unfold F in H5. rewrite H14 in H5.
+      inversion H5; subst.
+      dependent destruction H30.
+      unfold F in H15. rewrite H32 in H15.
+      inversion H15; subst.
+      dependent destruction H8.
+      unfold call, ret in x.
+      dependent destruction x.
+      rewrite ProgramFacts.frobProgId in x at 1. unfold ProgramFacts.frobProgram in x. simpl in x.
+      inversion x.
+      dependent destruction H1.
+      rewrite H29.
+      rewrite (ProgramFacts.frobProgId (@Return (CASSig bool) bool true;; Return tt)).
+      unfold ProgramFacts.frobProgram.
+      simpl. reflexivity.
+    }
+  + intros.
+    apply lemRet.
+    intros.
+    destruct v0.
+    easy.
+Qed.
+
+Lemma SpinLock_Acq_verified {T} : 
+  forall (i: Name T),
+    VerifyProg i (Rely i) (Guar i)
+      (prComp (Precs i unit Acq) (TInvoke SpinLockImpl i _ Acq) ->> Rely i)
+      (SpinLockImpl _ Acq)
+      (fun v => Posts i unit Acq v).
+Proof.
+  intros.
+  simpl.
+  unfold SpinLockAcq.
+Admitted.
+
+Lemma SpinLock_all_verified {T} : 
+  forall (i: Name T) A m,
+    VerifyProg i (Rely i) (Guar i)
+      (prComp (Precs i A m) (TInvoke SpinLockImpl i _ m) ->> Rely i)
+      (SpinLockImpl _ m)
+      (fun v => Posts i A m v).
+Proof.
+  intros.
+  destruct m eqn : I.
+  + apply SpinLock_Acq_verified.
+  + apply SpinLock_Rel_verified.
+Qed.
+
+End SpinLockNormal.
+
+
+
+
+Module SpinLockUB.
+
+Definition E := CASSig bool.
+Definition F := LockSig.
+Definition acf T := @LockActiveMap T.
+Definition HAcf T : @acf_sound T F lockSpec (acf T) := @LockActiveMapSound T.
+Definition VE T : Spec T E:= @casSpec T bool.
+Definition VF T := @lockSpec T.
+Definition VFU T := SpecWithUB (@lockSpec T) (acf T) (HAcf T).
+Definition ReltU T := Relt (VE T) (VFU T).
+Definition Relt T := Relt (VE T) (VF T).
+Definition PrecU T := Prec (VE T) (VFU T).
+Definition Prec T := Prec (VE T) (VF T).
+Definition PostU T := Post (VE T) (VFU T).
+Definition Post T := Post (VE T) (VF T).
+Definition UState T := State (VFU T).
+
+Definition Precs {T} i A (m : LockSig A) : @PrecU T :=
+  fun s ρs => exists ρ, ρs = eq ρ /\
+    match m with
+    | Acq =>
+        PState ρ = inl (LockOwned i) \/ 
+        PState ρ = inl (LockRelRan i) \/ 
+        PState ρ = inl (LockAcqRan i) \/
+        exists a, PState ρ = inr (UBState_, a)
+    | Rel =>
+        PState ρ <> inl (LockOwned i) /\
+        (StateWithUB_acf _ (acf T) (PState ρ) i = None)
+    end.
+
+Definition Posts {T} i A (m : LockSig A) : @PostU T A :=
+  fun _ s ρs t σs => exists ρ σ, ρs = eq ρ /\ σs = eq σ /\
+    match m with
+    | Acq =>
+        exists a, PState σ = inr (UBState_, a) /\
+        PCalls σ i = CallDone Acq /\
+        PRets σ i = RetPoss Acq tt
+    | Rel =>
+        exists a, PState σ = inr (UBState_, a) /\
+        PCalls σ i = CallDone Rel /\
+        PRets σ i = RetPoss Rel tt
+    end.
+
+(* Definition Rely {T} i := ReltWithUB (VF := (VF T)) (acf T) (HAcf T) (SpinLockNormal.Rely i).
+Definition Guar {T} i := ReltWithUB (VF := (VF T)) (acf T) (HAcf T) (SpinLockNormal.Guar i).
+Ltac unfold_rely H := unfold Rely, ReltWithUB, SpinLockNormal.Rely in H.
+Ltac unfold_guar H := unfold Guar, ReltWithUB, SpinLockNormal.Guar in H. *)
+
+Definition Rely {T} i : ReltU T :=
+  fun s ρs t σs => forall ρ, ρs = eq ρ -> exists σ, σs = eq σ /\
+    (PCalls ρ i = PCalls σ i) /\
+    (PRets ρ i = PRets σ i) /\
+    (forall m, PState ρ = inl (LockDef (Some i) m) -> 
+      (PState σ = inl (LockDef (Some i) m) \/ 
+      (exists a, PState σ = inr (UBState_, a)))) /\
+    True /\
+    (* (forall m, PState ρ = inl (LockDef (Some i) m) -> snd s = snd t) /\ *)
+    ((forall m, PState ρ <> inl (LockDef (Some i) m)) -> (forall m, PState σ <> inl (LockDef (Some i) m))) /\
+    ((exists a, PState ρ = inr (UBState_, a)) -> (exists a', PState σ = inr (UBState_, a'))) /\
+    (fst s i = fst t i) /\
+    (StateWithUB_acf _ (acf T) (PState ρ) i = StateWithUB_acf _ (acf T) (PState σ) i).
+
+Definition Guar {T} i : ReltU T :=
+  fun s ρs t σs => forall ρ, ρs = eq ρ -> exists σ, σs = eq σ /\
+    (forall j, j <> i -> fst s j = fst t j) /\
+    (forall j, j <> i -> PCalls ρ j = PCalls σ j) /\
+    (forall j, j <> i -> PRets ρ j = PRets σ j) /\
+    (forall j, j <> i ->
+      forall m, PState ρ = inl (LockDef (Some j) m) ->
+        (PState σ = inl (LockDef (Some j) m) \/ 
+        (exists a, PState σ = inr (UBState_, a)))) /\
+    True /\
+    (* (forall j, j <> i -> 
+      forall m, PState ρ = inl (LockDef (Some j) m) -> snd s = snd t) /\ *)
+    (forall j, j <> i -> 
+      ((forall m, PState ρ <> inl (LockDef (Some j) m)) -> (forall m, PState σ <> inl (LockDef (Some j) m)))) /\
+    ((exists a, PState ρ = inr (UBState_, a)) -> (exists a', PState σ = inr (UBState_, a'))) /\
+    (forall j, j <> i -> (StateWithUB_acf _ (acf T) (PState ρ) j = StateWithUB_acf _ (acf T) (PState σ) j)).
+
+Lemma Poss_eq_unique: forall {T} ρs (ρ: Poss (VFU T)) ρ', 
+  ρs = eq ρ -> ρs ρ' -> ρ = ρ'.
+Proof.
+  intros.
+  rewrite H in H0.
+  apply H0.
+Qed.
+
+Lemma Poss_eq_unique2: forall {T} ρs (ρ: Poss (VFU T)) ρ', 
+  ρs = eq ρ -> ρs = eq ρ' -> ρ' = ρ.
+Proof.
+  intros.
+  rewrite H in H0.
+  assert(eq ρ ρ = eq ρ' ρ). { rewrite H0. reflexivity. }
+  rewrite <- H1.
+  reflexivity.
+Qed.
+
+Lemma SpinLock_G_in_R {T} : 
+  forall (i j : Name T), i <> j -> Guar i ==> Rely j.
+Proof.
+  unfold Guar, Rely, sub, subRelt.
+  intros.
+  specialize (H0 _ H1).
+  destruct_all.
+  rename ρ into ρs.
+  rename σ into σs.
+  rename x into σ.
+  rename ρ0 into ρ.
+  exists σ.
+  assert(j <> i) by auto.
+  specialize (H2 _ H10).
+  specialize (H3 _ H10).
+  specialize (H4 _ H10).
+  specialize (H5 _ H10).
+  specialize (H7 _ H10).
+  specialize (H9 _ H10).
+  repeat split; intros; simpl; try easy.
+  + specialize (H5 _ H11).
+    destruct H5.
+    - left. easy.
+    - right. destruct_all. exists x. apply H5.
+  + specialize (H7 H11).
+    apply H7.
+  + apply (H8 H11).
+Qed.
+
+Lemma Rel_verify_aux1 {T} :
+  forall (i: Name T) (s0: InterState F (VE T)) (ρs0: PossSet (VFU T)) s1 ρs1,
+    (prComp (Precs i unit Rel) (TInvoke SpinLockImpl i unit Rel)) s0 ρs0 s1 ρs1 ->
+      exists ρ1, ρs1 = eq ρ1 /\
+        PState ρ1 <> inl (LockOwned i) /\
+        (StateWithUB_acf _ (acf T) (PState ρ1) i = None) /\
+        PCalls ρ1 i = CallPoss Rel /\
+        PRets ρ1 i = RetIdle /\
+        fst s1 i = Cont Rel (SpinLockImpl _ Rel).
+Proof.
+  intros.
+  unfold prComp, ReltCompose in H.
+  destruct H.
+  unfold Precs in H.
+  destruct H as [ρ0 [? ?]].
+  unfold TInvoke in H0.
+  destruct H0 as [? [? [? ?]]].
+  exists {| 
+    PState := ρ0.(PState); 
+    PCalls := fun j =>
+      if (eqb i j) then CallPoss Rel
+      else ρ0.(PCalls) j;
+    PRets := fun j =>
+      if (eqb i j) then RetIdle
+      else ρ0.(PRets) j
+  |}.
+  simpl.
+  rewrite (eqb_id i).
+  unfold TIdle in H0.
+  destruct H0.
+  split.
+  { pose proof SpinLockNormal.Poss_eq_inv i Rel ρs0 ρ0 ρs1
+    {| PState := PState ρ0; 
+       PCalls := fun j : Name T => if i =? j then CallPoss Rel else PCalls ρ0 j; 
+       PRets := fun j : Name T => if i =? j then RetIdle else PRets ρ0 j |} H H4.
+    apply H6.
+    reflexivity. }
+  repeat split; try easy.
+  inversion H2; subst; simpl in *.
+  inversion H6; subst.
+  dependent destruction H4.
+  exact H11.
+Qed.
+
+Lemma LockUnowned_Rely {T} :
+  forall (i: Name T) (s0: InterState F (VE T)) (ρs0: PossSet (VFU T)) s1 ρs1 ρ0,
+    ρs0 = eq ρ0 ->
+    Rely i s0 ρs0 s1 ρs1 ->
+    PState ρ0 <> inl (LockOwned i) ->
+    (exists ρ1, (ρs1 = eq ρ1) /\ PState ρ1 <> inl (LockOwned i)).
+Proof.
+  intros.
+  unfold Rely in H0.
+  specialize (H0 _ H).
+  destruct_all.
+  rename x into ρ1.
+  exists ρ1.
+  split; [exact H0 |].
+  destruct (PState ρ0).
+  + destruct s as [j m].
+    destruct j.
+    - rename n into j.
+      destruct (classicT (i = j)).
+      * subst j.
+        specialize (H4 m (ltac:(auto))).
+        destruct m.
+        { destruct H4.
+          rewrite H4. easy. 
+          destruct_all.
+          rewrite H4. easy.
+        }
+        contradiction.
+      * apply H6. intros. intro.
+        inversion H10. rewrite H12 in n. contradiction.
+    - apply H6. easy.
+  + assert(forall m : option (LockSig unit), inr p <> inl (LockDef (Some i) m)) by (intros; easy).
+    apply (H6 H10).
+Qed.
+
+Lemma Rel_verify_aux2 {T} :
+  forall (i: Name T) (s0: InterState F (VE T)) (ρs0: PossSet (VFU T)) s1 ρs1,
+    (prComp (Precs i unit Rel) (TInvoke SpinLockImpl i unit Rel) ->> Rely i) s0 ρs0 s1 ρs1 ->
+      exists ρ1, ρs1 = eq ρ1 /\
+        PState ρ1 <> inl (LockOwned i) /\
+        (StateWithUB_acf _ (acf T) (PState ρ1) i = None) /\
+        PCalls ρ1 i = CallPoss Rel /\
+        PRets ρ1 i = RetIdle /\
+        fst s1 i = Cont Rel (SpinLockImpl _ Rel).
+Proof.
+  intros.
+  unfold ReltCompose in H.
+  destruct H as [s2 [ρs2 [? ?]]].
+  pose proof Rel_verify_aux1 i s0 ρs0 s2 ρs2 H.
+  destruct H1 as [ρ2 [? [? [? [? ?]]]]].
+  pose proof LockUnowned_Rely _ _ _ _ _ _ H1 H0 H2.
+  unfold Rely in H0.
+  specialize (H0 _ H1).
+  destruct H0 as [ρ1 [? ?]].
+  destruct_all.
+  pose proof Poss_eq_unique2 _ _ _ H6 H0; subst x.
+  exists ρ1.
+  split; [exact H0 | ].
+  split; [exact H16 |].
+  split.
+  { rewrite <- H15. apply H3. }
+  split.
+  { rewrite <- H7. apply H4. }
+  split.
+  { rewrite <- H9. apply H5. }
+  rewrite <- H14. apply H8.
+Qed.
+
+Lemma Rel_verify_aux3 {T} :
+  forall (i: Name T) (s0: InterState F (VE T)) (ρs0: PossSet (VFU T)) s1 ρs1,
+    ((prComp (Precs i unit Rel) (TInvoke SpinLockImpl i unit Rel) ->> Rely i) ->>
+    (fun s ρs t σs =>
+        exists ρ σ, ρs = eq ρ /\ σs = eq σ /\
+        UnderThreadStep (fst s i) (Some (CallEv (CAS (Some true) None))) (fst t i) /\
+        (exists a, PState σ = inr (UBState_, a) /\ (a i = Some (existT (fun A => LockSig A) unit Rel))) /\
+        PCalls σ i = CallDone Rel /\
+        PRets σ i = RetIdle)) s0 ρs0 s1 ρs1 -> 
+    exists ρ1, ρs1 = eq ρ1 /\
+      (exists a, PState ρ1 = inr (UBState_, a) /\ (a i = Some (existT (fun A => LockSig A) unit Rel))) /\
+      PCalls ρ1 i = CallDone Rel /\
+      PRets ρ1 i = RetIdle /\
+      fst s1 i = UCall Rel (CAS (Some true) None) (fun x1 : bool => Return x1;; Return tt).
+Proof.
+  intros.
+  unfold ReltCompose in H at 1.
+  destruct H as [s2 [ρs2 [? ?]]].
+  pose proof Rel_verify_aux2 i s0 ρs0 s2 ρs2 H.
+  destruct H1 as [ρ2 [? [? [? [? ?]]]]].
+  destruct H0 as [ρ2' [ρ1 [? [? ?]]]].
+  pose proof Poss_eq_unique2 _ _ _ H0 H1; subst ρ2'.
+  exists ρ1.
+  split; [exact H6 |].
+  destruct_all.
+  split. { exists x. easy. }
+  split; [exact H10 |].
+  split; [exact H11 |].
+  rewrite H8 in H7.
+  inversion H7; subst.
+  dependent destruction H14.
+  unfold call, ret in x.
+  rewrite ProgramFacts.frobProgId in x at 1. unfold ProgramFacts.frobProgram in x. simpl in x.
+  inversion x.
+  dependent destruction H6.
+  rewrite H18.
+  reflexivity.
+Qed.
+
+Lemma Rel_verify_aux4 {T} :
+  forall (i: Name T) (s0: InterState F (VE T)) (ρs0: PossSet (VFU T)) s1 ρs1 v,
+    (((prComp (Precs i unit Rel) (TInvoke SpinLockImpl i unit Rel) ->> Rely i) ->>
+    (fun (s: InterState F (VE T)) (ρs: PossSet (VFU T)) t σs =>
+        exists ρ σ, ρs = eq ρ /\ σs = eq σ /\
+        UnderThreadStep (fst s i) (Some (CallEv (CAS (Some true) None))) (fst t i) /\
+        (exists a, PState σ = inr (UBState_, a) /\ (a i = Some (existT (fun A => LockSig A) unit Rel))) /\
+        PCalls σ i = CallDone Rel /\
+        PRets σ i = RetIdle)) ->>
+    (fun s ρs t (σs: PossSet (VFU T)) =>
+        exists ρ σ, ρs = eq ρ /\ σs = eq σ /\
+        UnderThreadStep (fst s i) (Some (RetEv (CAS (Some true) None) v)) (fst t i) /\
+        (exists a, PState σ = inr (UBState_, a) /\ a i = None) /\
+        PCalls σ i = CallDone Rel /\
+        PRets σ i = RetPoss Rel tt)) s0 ρs0 s1 ρs1 -> 
+    exists ρ1, ρs1 = eq ρ1 /\
+        fst s1 i = Cont Rel (Return tt) /\
+        (exists a, PState ρ1 = inr (UBState_, a) /\ a i = None) /\
+        PCalls ρ1 i = CallDone Rel /\
+        PRets ρ1 i = RetPoss Rel tt.
+Proof.
+  intros.
+  unfold ReltCompose in H at 1.
+  destruct H as [t [σs [? ?]]].
+  pose proof Rel_verify_aux3 i s0 ρs0 t σs H.
+  clear H.
+  destruct H1 as [σ [? ?]].
+  destruct_all.
+  rename x into a.
+  rename x0 into σ'.
+  rename x1 into ρ1.
+  pose proof Poss_eq_unique2 _ _ _ H0 H; subst σ'.
+  exists ρ1.
+  destruct_all.
+  split; [exact H6 |].
+  split.
+  { rewrite H4 in H7. inversion H7; subst.
+    dependent destruction H13.
+    dependent destruction H16.
+    rewrite H18.
+    rewrite (ProgramFacts.frobProgId (Return v;; Return tt)).
+    simpl. reflexivity.
+  }
+  split. { exists x2. easy. }
+  split; [exact H9 |].
+  exact H10.
+Qed.
+
+Lemma SpinLock_Rel_verified {T} : 
+  forall (i: Name T),
+    VerifyProg i (Rely i) (Guar i)
+      (prComp (Precs i unit Rel) (TInvoke SpinLockImpl i _ Rel) ->> Rely i)
+      (SpinLockImpl _ Rel)
+      (fun v => Posts i unit Rel v).
+Proof.
+  intros; simpl.
+  apply (lemBind (fun (_: bool) => 
+            (fun v : unit => Posts i unit Rel v) tt)).
+  + eapply weakenPost.
+    eapply (lemCall 
+      (Q := fun (s: InterState F (VE T)) (ρs: PossSet (VFU T)) t σs =>
+        exists ρ σ, ρs = eq ρ /\ σs = eq σ /\
+        UnderThreadStep (fst s i) (Some (CallEv (CAS (Some true) None))) (fst t i) /\
+        (* Step (VE T) (snd s) (i, (CallEv (CAS (Some true) None))) (snd t) /\  *)
+        (exists a, PState σ = inr (UBState_, a) /\ (a i = Some (existT (fun A => LockSig A) unit Rel))) /\
+        PCalls σ i = CallDone Rel /\
+        PRets σ i = RetIdle)
+      (S := fun v s ρs t σs =>
+        exists ρ σ, ρs = eq ρ /\ σs = eq σ /\
+        UnderThreadStep (fst s i) (Some (RetEv (CAS (Some true) None) v)) (fst t i) /\
+        (exists a, PState σ = inr (UBState_, a) /\ a i = None) /\
+        PCalls σ i = CallDone Rel /\
+        PRets σ i = RetPoss Rel tt)).
+    { unfold Stable, stableRelt, sub, subRelt, ReltCompose.
+      intros.
+      rename ρ into ρs.
+      rename σ into σs.
+      destruct H as [s1 [ρs1 ?]].
+      destruct H.
+      destruct H as [ρ [ρ1 [? [? ?]]]].
+      unfold Rely in H0.
+      specialize (H0 _ H1).
+      destruct H0 as [σ [? ?]].
+      exists ρ, σ.
+      split; [exact H |].
+      split; [exact H0 |].
+      destruct_all.
+      unfold F. rewrite <- H9.
+      split; [easy |].
+      split.
+      { assert((exists a : ActiveMap T LockSig, PState ρ1 = inr (UBState_, a))).
+        { exists x. easy. }
+        specialize (H8 H15).
+        destruct H8 as [a' ?].
+        exists a'.
+        split; [ easy |].
+        unfold F in H11. rewrite H11 in H10.
+        rewrite H8 in H10.
+        unfold StateWithUB_acf in H10.
+        rewrite <- H10.
+        apply H14.
+      }
+      rewrite <- H3, <- H4.
+      easy.
+    }
+    {
+      unfold Stable, stablePost, stableRelt, sub, subRelt, ReltCompose.
+      intros.
+      rename ρ into ρs.
+      rename σ into σs.
+      destruct H as [s1 [ρs1 ?]].
+      destruct H.
+      destruct H as [ρ [ρ1 [? [? ?]]]].
+      unfold Rely in H0.
+      specialize (H0 _ H1).
+      destruct H0 as [σ [? ?]].
+      exists ρ, σ.
+      split; [exact H |].
+      split; [exact H0 |].
+      destruct_all.
+      unfold F. rewrite <- H9.
+      split; [easy |].
+      split.
+      { assert((exists a : ActiveMap T LockSig, PState ρ1 = inr (UBState_, a))).
+        { exists x. easy. }
+        specialize (H8 H15).
+        destruct H8 as [a' ?].
+        exists a'.
+        split; [ easy |].
+        unfold F in H11. rewrite H11 in H10.
+        rewrite H8 in H10.
+        unfold StateWithUB_acf in H10.
+        rewrite <- H10.
+        apply H14.
+      }
+      rewrite <- H3, <- H4.
+      easy.
+    }
+    {
+      unfold Commit.
+      intros.
+      unfold ReltToPrec in H.
+      destruct H as [s0 [ρs0 ?]].
+      pose proof Rel_verify_aux2 i s0 ρs0 s ρs H.
+      destruct H3 as [ρ [? [? [? [? ?]]]]].
+      remember (
+        MkPoss T F (VFU T)
+        (inr (UBState_, fun j => if i =? j then Some (existT (fun A => LockSig A) unit Rel) else (StateWithUB_acf _ (acf T) (PState ρ) j)))
+        (fun j => if i =? j then CallDone Rel else PCalls ρ j)
+        (fun j => if i =? j then RetIdle else PRets ρ j)) as σ.
+      exists (eq σ).
+      split. { exists σ. reflexivity. }
+      split.
+      { intros. exists ρ.
+        split. { rewrite H3. reflexivity. }
+        subst σ0.
+        apply (PossStepsStep i ρ σ σ).
+        { apply (PCommitCall i _ _ unit Rel); subst σ; simpl; try easy.
+          { destruct (PState ρ).
+            { constructor.
+              { intros. intro. inversion H8; subst. contradiction. }
+              { constructor. 
+                { unfold StateWithUB_acf in H5. apply H5. }
+                { rewrite eqb_id. reflexivity. }
+                { apply differ_pointwise_trivial. }
+              }
+            }
+            { destruct p. destruct u. constructor. constructor.
+              { unfold StateWithUB_acf in H5. apply H5. }
+              { rewrite eqb_id. reflexivity. }
+              { apply differ_pointwise_trivial. }
+            }
+          }
+          { rewrite eqb_id. reflexivity. }
+          { rewrite eqb_id. reflexivity. }
+        }
+        { intros. subst σ. simpl. rewrite (eqb_nid _ _ H8). reflexivity. }
+        { intros. subst σ. simpl. rewrite (eqb_nid _ _ H8). reflexivity. }
+        { constructor. }
+      }
+      split.
+      { exists ρ, σ.
+        repeat split; subst σ; simpl; try rewrite eqb_id; try easy.
+        eexists.
+        split. { reflexivity. }
+        simpl. rewrite eqb_id. reflexivity.
+      }
+      { unfold Guar.
+        intros.
+        pose proof Poss_eq_unique2 _ _ _ H8 H3; subst ρ0.
+        exists σ.
+        split; [reflexivity |].
+        split. 
+        { intros. unfold differ_pointwise in H0. specialize (H0 _ H9). easy. }
+        split.
+        { subst σ. simpl. intros. rewrite (eqb_nid i j (ltac:(auto))). reflexivity. }
+        split.
+        { subst σ. simpl. intros. rewrite (eqb_nid i j (ltac:(auto))). reflexivity. }
+        split.
+        { intros. subst σ. simpl.
+          right. 
+          eexists. reflexivity.
+        }
+        split; [ easy |].
+        split. { intros. subst σ. easy. }
+        split.
+        { intros. subst σ. simpl. eexists. reflexivity. }
+        { intros. subst σ. simpl. rewrite (eqb_nid i j (ltac:(auto))). reflexivity. }
+      }
+    }
+    {
+      unfold Commit.
+      intros.
+      unfold ReltToPrec in H.
+      destruct H as [s0 [ρs0 ?]].
+      pose proof Rel_verify_aux3 i s0 ρs0 s ρs H.
+      clear H.
+      destruct H3 as [ρ [? [? [? [? ?]]]]].
+      destruct H3 as [a [? ?]].
+      remember (
+        MkPoss T F (VFU T)
+        (inr (UBState_, fun j => if i =? j then None else (StateWithUB_acf _ (acf T) (PState ρ) j)))
+        (fun j => if i =? j then CallDone Rel else PCalls ρ j)
+        (fun j => if i =? j then RetPoss Rel tt else PRets ρ j)) as σ.
+      exists (eq σ).
+      split. { exists σ. reflexivity. }
+      split.
+      { intros. exists ρ.
+        split. { rewrite H. reflexivity. }
+        subst σ0.
+        apply (PossStepsStep i ρ σ σ).
+        { apply (PCommitRet i _ _ unit Rel tt); subst σ; simpl; try easy.
+          { rewrite H3. constructor. constructor.
+            { apply H7. }
+            { rewrite eqb_id. reflexivity. }
+            { apply differ_pointwise_trivial. }
+        }
+        { rewrite eqb_id. reflexivity. }
+        { rewrite eqb_id. reflexivity. }
+        }
+        { intros. subst σ. simpl. rewrite (eqb_nid _ _ H8). reflexivity. }
+        { intros. subst σ. simpl. rewrite (eqb_nid _ _ H8). reflexivity. }
+        { constructor. }
+      }
+      split.
+      { exists ρ, σ.
+        unfold F in H1. rewrite H6 in H1. inversion H1; subst.
+        dependent destruction H9.
+        dependent destruction H12.
+        unfold F. rewrite H6.
+        repeat split; simpl; try rewrite eqb_id; try easy.
+        eexists. split; [reflexivity |].
+        simpl. rewrite eqb_id. reflexivity.
+      }
+      { unfold Guar.
+        intros.
+        pose proof Poss_eq_unique2 _ _ _ H8 H; subst ρ0.
+        exists σ.
+        split; [reflexivity |].
+        split. 
+        { intros. unfold differ_pointwise in H0. specialize (H0 _ H9). easy. }
+        split.
+        { subst σ. simpl. intros. rewrite (eqb_nid i j (ltac:(auto))). reflexivity. }
+        split.
+        { subst σ. simpl. intros. rewrite (eqb_nid i j (ltac:(auto))). reflexivity. }
+        split.
+        { intros. subst σ. simpl.
+          right. 
+          eexists. reflexivity.
+        }
+        split; [ easy |].
+        split. { intros. subst σ. easy. }
+        split.
+        { intros. subst σ. simpl. eexists. reflexivity. }
+        { intros. subst σ. simpl. rewrite (eqb_nid i j (ltac:(auto))). reflexivity. }
+      }
+    }
+    {
+      unfold sub, subRelt.
+      intros.
+      rename ρ into ρs.
+      rename σ into σs.
+      rewrite <- LogicFacts.reltCompAssoc in H.
+      pose proof Rel_verify_aux4 i s ρs t σs v H.
+      assert(exists ρ, ρs = eq ρ).
+      { unfold ReltCompose in H. destruct_all. unfold prComp in H.
+        destruct H.
+        unfold Precs in H.
+        destruct H as [ρ0 [? ?]].
+        exists ρ0. rewrite H. reflexivity. 
+      }
+      clear H.
+      destruct H0 as [σ [? ?]].
+      unfold Posts.
+      destruct H1 as [ρ ?].
+      destruct_all.
+      exists ρ, σ.
+      repeat split; try easy.
+      exists x. easy.
+    }
+  + intros.
+    constructor.
+    easy. 
+Qed.
+
+End SpinLockUB.
+
+Module SpinLockAll.
+
